a simple example that prints some strings.

tests/c-test/main_c_spec.v
@@ -9,38 +9,23 @@ From Cpp Require Import
      Auto.
 
 Require C.main_c.
+Require Import C.array.
 
-Definition Vchar (a : Ascii.ascii) : val :=
-  Vint (Z.of_N (N_of_ascii a)).
+Definition args_array (p : val) (ls : list string) : mpred :=
+  tarray (Tpointer (Qmut T_char))
+    (fun (p : val) (v : string) =>
+       Exists s : val,
+         tptsto (Tpointer (Qmut T_char)) p s ** c_string s v) p
+    ls.
 
 
-
-(* representation of c-style strings, i.e. null-terminated *)
-Fixpoint c_string (p : val) (ls : string) : mpred :=
-  match ls with
-  | EmptyString => tptsto T_schar p (Vchar "000"%char)
-  | String c cs =>
-    tptsto T_schar p (Vchar c) **
-    c_string (offset_ptr p 1) cs
-  end.
-
-Section array.
-  Context {T : Type}.
-  Variable sz : Z.
-  Variable (P : val -> T -> mpred).
-  Fixpoint array' (p : val) (ls : list T) : mpred :=
-    match ls with
-    | nil => empSP
-    | l :: ls =>
-      P p l ** array' (offset_ptr p sz) ls
-    end.
-End array.
-
-(* typed arrays *)
-Definition tarray (t : type) {T : Type} (P : val -> T -> mpred)
-           (base : val) (ls : list T) : mpred :=
-  Exists sz, with_genv (fun g => [| @size_of g t sz |]) **
-             array' sz P base ls.
+Definition putstr_spec : function_spec' :=
+  SFunction (Qmut Tvoid) (Qmut (Tpointer (Qmut T_char)) :: nil)
+            (fun p =>
+               {| wpp_with := string
+                ; wpp_pre s := c_string p s
+                ; wpp_post s _ := c_string p s
+                |}).
 
 Definition main_spec : function_spec' :=
   SFunction (Qmut T_int)
@@ -48,21 +33,18 @@ Definition main_spec : function_spec' :=
                   (Qconst (Tpointer
                              (Qmut
                                 (Tpointer
-                                   (Qmut (Tchar (Some 8%nat) true)))))) :: nil)
+                                   (Qmut T_char))))) :: nil)
       (fun argc argv =>
          {| wpp_with := list string
           ; wpp_pre m :=
               [| Vint (Z.of_nat (length m)) = argc |] **
-              tarray (Tpointer (Qmut (Tchar (Some 8%nat) true)))
-                     (fun p v =>
-                        Exists s, tptsto (Tpointer (Qmut (Tchar (Some 8%nat) true))) p s ** c_string p v)
-                     argv m
-          ; wpp_post m (r : val) := [| r = Vint 3 |] **
-              tarray (Tpointer (Qmut (Tchar (Some 8%nat) true)))
-                     (fun p v =>
-                        Exists s, tptsto (Tpointer (Qmut (Tchar (Some 8%nat) true))) p s ** c_string p v)
-                     argv m
+              args_array argv m
+          ; wpp_post m (r : val) := [| r = Vint 0 |] **
+              args_array argv m
          |}).
 
-Definition main_cpp_spec (resolve : _) :=
+Definition spec (resolve : _) :=
+  ti_cglob' (resolve:=resolve) "_Z6putstr" putstr_spec -*
   ti_cglob' (resolve:=resolve) "_Z4main" main_spec.
+
+Export C.array.
