tests/c-test/main_c_proof.v
@@ -1,0 +1,97 @@
+Require Import Coq.ZArith.BinInt.
+Require Import Coq.Strings.String.
+
+Local Open Scope Z_scope.
+Local Open Scope string_scope.
+
+From ChargeCore.Logics Require Import
+     ILogic BILogic ILEmbed Later.
+
+From Cpp Require Import
+     Auto.
+
+Require C.main_c.
+Require Import C.main_c_spec.
+
+
+Lemma can_get_element {T} :
+  forall (x3 : list T) (x4 : Z),
+    0 <= x4 <= Z.of_nat (Datatypes.length x3) ->
+    x4 < Z.of_nat (Datatypes.length x3) ->
+    exists (v : T) (i : nat), Z.of_nat i = x4 /\ nth_error x3 i = Some v.
+Proof. Admitted.
+
+(* soundness of the specification *)
+Theorem main_cpp_sound : forall (resolve : genv),
+    denoteModule main_c.module |-- spec resolve.
+Proof.
+  intros.
+  simpl.
+  unfold spec.
+  start_module.
+
+  verifyF_forget "_Z4main".
+  { (* ::main(int argc, char* argv[]) *)
+    start_proof.
+    rewrite denoteModule_weaken.
+    simplifying.
+    work.
+    (* this is the loop invariant
+     * todo(gmm): i need to clean this up a lot!
+     *)
+    transitivity (
+        (ti_cglob' (resolve:=resolve) "_Z6putstr" putstr_spec **
+         tlocal x1 (Tint None true) "argc" x **
+         tlocal x1 (Tpointer (Qmut (Tpointer (Qmut T_char)))) "argv" x0) **
+         (Forall res : val, [| res = 0 |] ** args_array x0 x3 -* x2 res) **
+         args_array x0 x3 **
+         Exists i,
+           [| 0 <= i <= Z.of_nat (Datatypes.length x3) |] **
+           tlocal x1 T_int "i" i).
+    { work. }
+    eapply wp_for.
+    simplifying.
+    work.
+    simplifying.
+    work.
+    { simpl.
+      eapply embedPropR.
+      eapply eval_lt; try reflexivity. subst. reflexivity. }
+    rewrite is_true_int.
+    destruct (ZArith_dec.Z_lt_ge_dec x4 (Z.of_nat (Datatypes.length x3))).
+    { simpl.
+      simplifying.
+      unfold args_array.
+      assert (exists v, exists i, Z.of_nat i = x4 /\ nth_error x3 i = Some v).
+      { eapply can_get_element; eauto. }
+      destruct H1 as [ ? [ ? [ ? ? ] ] ].
+      rewrite tarray_cell; eauto with size_of.
+      rewrite <- wp_lhs_subscript.
+      simplifying.
+      simpl.
+      work.
+      simplifying.
+      work.
+      { subst. work. }
+      simplifying. simpl.
+      unfold tlocal.
+      lift_ex_l.
+      perm_left ltac:(idtac; eapply (Lemmas.learn_bounds x4); simpl; intros).
+      work.
+      instantiate (1:=Vint (x4 + 1)).
+      eapply provable_star.
+      { eapply eval_add. reflexivity.
+        eapply has_type_int_any. }
+      work.
+      rewrite tarray_cell with (ms:=x3); eauto with size_of.
+      work. }
+    { simpl.
+      unfold Sskip.
+      simplifying.
+      work.
+      done_proof. } }
+
+  finish_module.
+  Unshelve.
+  all: eassumption.
+Qed.
