theories/Sem/Semantics.v
@@ -46,13 +46,53 @@ Hint Resolve has_type_int_any has_type_int_bound has_type_qual
 Parameter eval_unop : UnOp -> type -> val -> val -> Prop.
 Parameter eval_binop : BinOp -> type -> val -> val -> val -> Prop.
 
-Lemma eval_add : forall ty (a b c : Z),
-    c = (Z.add a b) ->
-    has_type (Vint c) ty ->
-    eval_binop Badd ty (Vint a) (Vint b) (Vint c).
-Proof using. Admitted.
+Definition eval_int_op (bo : BinOp) (o : Z -> Z -> Z) : Prop :=
+  forall w s (a b c : Z),
+    c = o a b ->
+    has_type (Vint c) (Tint w s) ->
+    eval_binop bo (Tint w s) (Vint a) (Vint b) (Vint c).
+
+Axiom eval_add :
+  ltac:(let x := eval hnf in (eval_int_op Badd Z.add) in refine x).
+Axiom eval_sub :
+  ltac:(let x := eval hnf in (eval_int_op Bsub Z.sub) in refine x).
+Axiom eval_ :
+  ltac:(let x := eval hnf in (eval_int_op Bmul Z.mul) in refine x).
+Axiom eval_div :
+  ltac:(let x := eval hnf in (eval_int_op Bdiv Z.div) in refine x).
+Axiom eval_mod :
+  ltac:(let x := eval hnf in (eval_int_op Bmod Z.modulo) in refine x).
+
+Definition eval_int_rel_op (bo : BinOp) {P Q : Z -> Z -> Prop}
+           (o : forall a b : Z, {P a b} + {Q a b}) : Prop :=
+  forall w s a b (av bv : Z) (c : Z),
+    a = Vint av ->
+    b = Vint bv ->
+    c = (if o av bv then 1 else 0)%Z ->
+    eval_binop bo (Tint w s) a b (Vint c).
+
+Axiom eval_eq :
+  ltac:(let x := eval hnf in (eval_int_rel_op Beq Z.eq_dec) in refine x).
+Axiom eval_neq :
+  forall ty a b (av bv : Z) (c : Z),
+    a = Vint av ->
+    b = Vint bv ->
+    c = (if Z.eq_dec av bv then 0 else 1)%Z ->
+    eval_binop Bneq ty a b (Vint c).
+Axiom eval_lt :
+  ltac:(let x := eval hnf in (eval_int_rel_op Blt ZArith_dec.Z_lt_ge_dec) in refine x).
+Axiom eval_gt :
+  ltac:(let x := eval hnf in (eval_int_rel_op Bgt ZArith_dec.Z_gt_le_dec) in refine x).
+Axiom eval_le :
+  ltac:(let x := eval hnf in (eval_int_rel_op Ble ZArith_dec.Z_le_gt_dec) in refine x).
+Axiom eval_ge :
+  ltac:(let x := eval hnf in (eval_int_rel_op Bge ZArith_dec.Z_ge_lt_dec) in refine x).
 
 Parameter offset_ptr : val -> Z -> val.
+Axiom offset_ptr_combine : forall b o o',
+    offset_ptr (offset_ptr b o) o' = offset_ptr b (o + o').
+Axiom offset_ptr_0 : forall b,
+    offset_ptr b 0 = b.
 
 Parameter is_true : val -> bool.
 Axiom is_true_int : forall i,
